core/Peo.v
@@ -16,13 +16,13 @@ Definition are_neighbors (r : reg) (regs : list reg) (g : ig) : bool :=
     (fun b r' =>
       b &&
       ((r =? r') ||
-        regs_mem r' (dict_map g r)))
+        regs_mem r' (ig_map g r)))
     regs
     true
 .
 
 Definition is_simplicial (r : reg) (g : ig) : bool :=
-  let regs := dict_map g r in
+  let regs := ig_map g r in
   regs_mem r (dict_keys g) &&
   fold_left (* Check whether the neighbor set of r is a clique *)
     (fun b r =>
@@ -33,30 +33,46 @@ Definition is_simplicial (r : reg) (g : ig) : bool :=
     true
 .
 
-Definition find_next (g : ig) : option reg :=
-  let fix find_next_aux (regs : list reg) : option reg :=
-    match regs with
-    | nil => None
-    | r :: rs =>
-      if is_simplicial r g then Some r else find_next_aux rs
-    end
-  in
-  find_next_aux (dict_keys g)
-.
-
-(*
-  We need to use `vreg` instead of `reg` for the OCaml extraction
-*)
-Fixpoint eliminate (g : ig) (fuel : nat) : ig * list vreg :=
-  match fuel with
-  | O => (g, nil)
-  | S fuel' =>
-    match find_next g with
-    | Some next =>
-      let g' := ig_remove_node g next in
-      let (g'', peo) := eliminate g' fuel' in
-      (g'', next :: peo)
-    | None => (g, nil)
-    end
+Fixpoint find_next_aux (regs : list reg) (g : ig) : option reg :=
+  match regs with
+  | nil => None
+  | r :: rs =>
+    if is_simplicial r g then Some r else find_next_aux rs g
   end
 .
+
+Definition find_next (g : ig) : option reg :=
+  find_next_aux (dict_keys g) g
+. 
+
+Lemma find_next_mem :
+  forall (g : ig) (n : reg), find_next g = Some n -> In n (dict_keys g)
+.
+Proof.
+  intros g n H. unfold find_next in H. generalize dependent n.
+  induction (dict_keys g) as [|r rs IH].
+  - intros n'. simpl. congruence.
+  - intros n'. simpl.
+    destruct (is_simplicial r g).
+    + intros H. injection H. intro H0. left. assumption.
+    + intros H. apply IH in H. right. assumption.
+Qed.
+
+From Stdlib Require Import FunInd.
+From Stdlib Require Import Recdef.
+
+Function eliminate (g : ig) {measure dict_size g} : ig * list vreg :=
+  match find_next g with
+  | Some next =>
+    let g' := ig_remove_node g next in
+    let (g'', peo) := eliminate g' in
+    (g'', next :: peo)
+  | None => (g, nil)
+  end
+.
+Proof.
+  intros g n H.
+  apply find_next_mem in H.
+  apply dict_size_decrease.
+  assumption.
+Qed.
